feat: equivalents of Church-Rosser, some normal form properties (#215)
This is work from the ItaLean conference by myself, @XYUnknown,
@a-dangelo, and @Aristotle-Harmonic. I made the decision here to move
this file into only extending the existing `Relation` namespace which I
think is much clearer. I also cleaned up some names for style
consistency.

---------

Co-authored-by: ADA <120643053+ADA-Projects@users.noreply.github.com>
Co-authored-by: Xueying Qin <32066429+XYUnknown@users.noreply.github.com>
Co-authored-by: Aristotle Harmonic <aristotle-harmonic@harmonic.fun>

Cslib/Foundations/Data/Relation.lean
@@ -6,80 +6,145 @@ Authors: Fabrizio Montesi, Thomas Waring, Chris Henson
 
 import Cslib.Init
 import Mathlib.Logic.Relation
+import Mathlib.Data.List.TFAE
 
 /-! # Relations -/
 
-namespace Cslib
+namespace Relation
 
-universe u v
+variable {α : Type*} {r : α → α → Prop}
 
-section Relation
+attribute [scoped grind] ReflGen TransGen ReflTransGen EqvGen
+
+theorem ReflGen.to_eqvGen (h : ReflGen r a b) : EqvGen r a b := by
+  induction h <;> grind
+
+theorem TransGen.to_eqvGen (h : TransGen r a b) : EqvGen r a b := by
+  induction h <;> grind
+
+theorem ReflTransGen.to_eqvGen (h : ReflTransGen r a b) : EqvGen r a b := by
+  induction h <;> grind
+
+attribute [scoped grind →] ReflGen.to_eqvGen TransGen.to_eqvGen ReflTransGen.to_eqvGen
 
 /-- The relation `r` 'up to' the relation `s`. -/
-def Relation.UpTo (r s : α → α → Prop) : α → α → Prop := Relation.Comp s (Relation.Comp r s)
+def UpTo (r s : α → α → Prop) : α → α → Prop := Comp s (Comp r s)
 
 /-- A relation has the diamond property when all reductions with a common origin are joinable -/
-abbrev Diamond (R : α → α → Prop) := ∀ {A B C : α}, R A B → R A C → (∃ D, R B D ∧ R C D)
+abbrev Diamond (r : α → α → Prop) := ∀ {A B C : α}, r A B → r A C → Join r B C
 
 /-- A relation is confluent when its reflexive transitive closure has the diamond property. -/
-abbrev Confluence (R : α → α → Prop) := Diamond (Relation.ReflTransGen R)
+abbrev Confluent (r : α → α → Prop) := Diamond (ReflTransGen r)
 
-open _root_.Relation _root_.Relation.ReflTransGen in
+/-- A relation is semi-confluent when single and multiple steps with common origin
+  are multi-joinable. -/
+abbrev SemiConfluent (r : α → α → Prop) :=
+  ∀ {x y₁ y₂}, ReflTransGen r x y₂ → r x y₁ → Join (ReflTransGen r) y₁ y₂
+
+/-- A relation has the Church Rosser property when equivalence implies multi-joinability. -/
+abbrev ChurchRosser (r : α → α → Prop) := ∀ {x y}, EqvGen r x y → Join (ReflTransGen r) x y
+
 /-- Extending a multistep reduction by a single step preserves multi-joinability. -/
-lemma Relation.ReflTransGen.diamond_extend (h : Diamond R) :
-  ReflTransGen R A B →
-  R A C →
-  ∃ D, Relation.ReflTransGen R B D ∧ Relation.ReflTransGen R C D := by
-  intros AB _
-  revert C
-  induction AB using Relation.ReflTransGen.head_induction_on <;> intros C AC
-  case refl => exact ⟨C, ⟨single AC, by rfl⟩⟩
+lemma Diamond.extend (h : Diamond r) :
+    ReflTransGen r A B → r A C → Join (ReflTransGen r) B C := by
+  intros AB AC
+  induction AB using ReflTransGen.head_induction_on generalizing C
+  case refl => exists C, .single AC
   case head A'_C' _ ih =>
-    obtain ⟨D, ⟨CD, C'_D⟩⟩ := h AC A'_C'
-    obtain ⟨D', ⟨B_D', D_D'⟩⟩ := ih C'_D
-    exact ⟨D', ⟨B_D', head CD D_D'⟩⟩
+    obtain ⟨D, CD, C'_D⟩ := h AC A'_C'
+    obtain ⟨D', B_D', D_D'⟩ := ih C'_D
+    exact ⟨D', B_D', .head CD D_D'⟩
 
-open _root_.Relation _root_.Relation.ReflTransGen in
 /-- The diamond property implies confluence. -/
-theorem Relation.ReflTransGen.diamond_confluence (h : Diamond R) : Confluence R := by
+theorem Diamond.toConfluent (h : Diamond r) : Confluent r := by
   intros A B C AB BC
-  revert C
-  induction AB using head_induction_on <;> intros C BC
+  induction AB using ReflTransGen.head_induction_on generalizing C
   case refl => exists C
   case head _ _ A'_C' _ ih =>
-    obtain ⟨D, ⟨CD, C'_D⟩⟩ := diamond_extend h BC A'_C'
-    obtain ⟨D', ⟨B_D', D_D'⟩⟩ := ih C'_D
-    exact ⟨D', ⟨B_D', ReflTransGen.trans CD D_D'⟩⟩
+    obtain ⟨D, CD, C'_D⟩ := h.extend BC A'_C'
+    obtain ⟨D', B_D', D_D'⟩ := ih C'_D
+    exact ⟨D', B_D', .trans CD D_D'⟩
 
--- not sure why this doesn't compile as an "instance" but oh well
+theorem Confluent.toChurchRosser (h : Confluent r) : ChurchRosser r := by
+  intro x y h_eqv
+  induction h_eqv with
+  | rel _ b => exists b; grind [ReflTransGen.single]
+  | refl a => exists a
+  | symm a b _ ih => exact symmetric_join ih
+  | trans _ _ _ _ _ ih1 ih2 =>
+      obtain ⟨u, _, hbu⟩ := ih1
+      obtain ⟨v, hbv, _⟩ := ih2
+      obtain ⟨w, _, _⟩ := h hbu hbv
+      exists w
+      grind [ReflTransGen.trans]
+
+theorem SemiConfluent.toConfluent (h : SemiConfluent r) : Confluent r := by
+  intro x y1 y2 h_xy1 h_xy2
+  induction h_xy1 with
+  | refl => use y2
+  | tail h_xz h_zy1 ih =>
+      obtain ⟨u, h_zu, _⟩ := ih
+      obtain ⟨v, _, _⟩ := h h_zu h_zy1
+      exists v
+      grind [ReflTransGen.trans]
+
+attribute [scoped grind →] Confluent.toChurchRosser SemiConfluent.toConfluent
+
+private theorem confluent_equivalents : [ChurchRosser r, SemiConfluent r, Confluent r].TFAE := by
+  grind [List.tfae_cons_cons, List.tfae_singleton]
+
+theorem SemiConfluent_iff_ChurchRosser : SemiConfluent r ↔ ChurchRosser r :=
+  List.TFAE.out confluent_equivalents 1 0
+
+theorem Confluent_iff_ChurchRosser : Confluent r ↔ ChurchRosser r :=
+  List.TFAE.out confluent_equivalents 2 0
+
+theorem Confluent_iff_SemiConfluent : Confluent r ↔ SemiConfluent r :=
+  List.TFAE.out confluent_equivalents 2 1
+
+/-- An element is reducible with respect to a relation if there is a value it is related to. -/
+abbrev Reducible (r : α → α → Prop) (x : α) : Prop := ∃ y, r x y
+
+/-- An element is normal if it is not reducible. -/
+abbrev Normal (r : α → α → Prop) (x : α) : Prop := ¬ Reducible r x
+
+/-- A multi-step from a normal form must be reflexive. -/
+@[grind =>]
+theorem Normal.reflTransGen_eq (h : Normal r x) (xy : ReflTransGen r x y) : x = y := by
+  induction xy <;> grind
+
+/-- For a Church-Rosser relation, elements in an equivalence class must be multi-step related. -/
+theorem ChurchRosser.normal_eqvGen_reflTransGen (cr : ChurchRosser r) (norm : Normal r x)
+    (xy : EqvGen r y x) : ReflTransGen r y x := by
+  have ⟨_, _, _⟩ := cr xy
+  grind
+
+/-- For a Church-Rosser relation there is one normal form in each equivalence class. -/
+theorem ChurchRosser.normal_eq (cr : ChurchRosser r) (nx : Normal r x) (ny : Normal r y)
+    (xy : EqvGen r x y) : x = y := by
+  have ⟨_, _, _⟩ := cr xy
+  grind
+
 /-- A pair of subrelations lifts to transitivity on the relation. -/
-def trans_of_subrelation {α : Type*} (s s' r : α → α → Prop) (hr : Transitive r)
-    (h : ∀ a b : α, s a b → r a b) (h' : ∀ a b : α, s' a b → r a b) : Trans s s' r where
-  trans hab hbc := hr (h _ _ hab) (h' _ _ hbc)
+def trans_of_subrelation (s s' r : α → α → Prop) (hr : Transitive r)
+    (h : Subrelation s r) (h' : Subrelation s' r) : Trans s s' r where
+  trans hab hbc := hr (h hab) (h' hbc)
 
 /-- A subrelation lifts to transitivity on the left of the relation. -/
-def trans_of_subrelation_left {α : Type*} (s r : α → α → Prop) (hr : Transitive r)
-    (h : ∀ a b : α, s a b → r a b) : Trans s r r where
-  trans hab hbc := hr (h _ _ hab) hbc
+def trans_of_subrelation_left (s r : α → α → Prop) (hr : Transitive r)
+    (h : Subrelation s r) : Trans s r r where
+  trans hab hbc := hr (h hab) hbc
 
 /-- A subrelation lifts to transitivity on the right of the relation. -/
-def trans_of_subrelation_right {α : Type*} (s r : α → α → Prop) (hr : Transitive r)
-    (h : ∀ a b : α, s a b → r a b) : Trans r s r where
-  trans hab hbc := hr hab (h _ _ hbc)
+def trans_of_subrelation_right (s r : α → α → Prop) (hr : Transitive r)
+    (h : Subrelation s r) : Trans r s r where
+  trans hab hbc := hr hab (h hbc)
 
-/-- This is a straightforward but useful specialisation of a more general result in
-`Mathlib.Logic.Relation`. -/
-theorem church_rosser_of_diamond {α : Type*} {r : α → α → Prop}
-    (h : ∀ a b c, r a b → r a c → Relation.Join r b c) :
-    Equivalence (Relation.Join (Relation.ReflTransGen r)) := by
-  apply Relation.equivalence_join_reflTransGen
+/-- The diamond property implies that multi-step joinability is an equivalence. -/
+theorem Diamond.equivalence_join_reflTransGen (h : Diamond r) :
+    Equivalence (Join (ReflTransGen r)) := by
+  apply Relation.equivalence_join reflexive_reflTransGen transitive_reflTransGen
   intro a b c hab hac
-  let ⟨d, hd⟩ := h a b c hab hac
-  use d
-  constructor
-  · exact Relation.ReflGen.single hd.1
-  · exact Relation.ReflTransGen.single hd.2
+  exact h.toConfluent hab hac
 
 end Relation
-
-end Cslib
